Test/Passes/InstructionSelection/RISCV64/icmp_invalid.mlir
@@ -9,8 +9,5 @@
         // CHECK-NEXT:      "llvm.icmp"(%{{.*}}, %{{.*}}) <{"predicate" = 2 : i64}> : (i32, i32) -> i1
         %r_6 = "llvm.icmp"(%c, %b) <{"predicate" = 6 : i64}> : (i64, i32) -> i1
         // CHECK-NEXT:      "llvm.icmp"(%{{.*}}, %{{.*}}) <{"predicate" = 6 : i64}> : (i64, i32) -> i1
-        %r_11 = "llvm.icmp"(%c, %c) <{"predicate" = 11 : i64}> : (i64, i64) -> i1
-        // CHECK-NEXT:      "llvm.icmp"(%{{.*}}, %{{.*}}) <{"predicate" = 11 : i64}> : (i64, i64) -> i1
   }) : () -> ()
 }) : () -> ()
-
